{
 "cells": [
  {
   "cell_type": "markdown",
   "id": "8b855790",
   "metadata": {},
   "source": [
    "# MAT-MEK4270 Oblig 1"
   ]
  },
  {
   "cell_type": "markdown",
   "id": "1f3c68d5",
   "metadata": {},
   "source": [
    "## Exercise 1.2.3\n",
    "\n",
    "We want to show that \n",
    "\n",
    "\\begin{equation}\n",
    "u(t, x, y) = e^{i(k_x x + k_y y - \\omega t)}\n",
    "\\end{equation}\n",
    "\n",
    "satisfies the wave equation $u_{tt} = c^2(u_{xx} + u_{yy})$\n",
    "\n",
    "We start by finding $u_{tt}$, $u_{xx}$ and $u_{yy}$:\n",
    "\n",
    "$$\n",
    "u_{tt} = \\frac{\\partial^2 u}{\\partial t^2}(e^{i(k_x x + k_y y - \\omega t)}) = -\\omega^2 e^{i(k_x x + k_y y - \\omega t)}\\\\\n",
    "$$\n",
    "$$\n",
    "u_{xx} = \\frac{\\partial^2 u}{\\partial x^2}(e^{i(k_x x + k_y y - \\omega t)}) = -k_x^2 e^{i(k_x x + k_y y - \\omega t)}\n",
    "$$\n",
    "$$\n",
    "u_{yy} = \\frac{\\partial^2 u}{\\partial y^2}(e^{i(k_x x + k_y y - \\omega t)}) = -k_y^2 e^{i(k_x x + k_y y - \\omega t)}\n",
    "$$\n",
    "\n",
    "We can now substitute into the wave equation:\n",
    "\n",
    "$$\n",
    "-\\omega^2u = -c^2 (k_x^2 + k_y^2)u.\n",
    "$$\n",
    "\n",
    "Since u never is equal to 0, we can cancel out u and we get:\n",
    "\n",
    "$$\n",
    "\\omega^2 = c^2 (k_x^2 + k_y^2),\n",
    "$$\n",
    "\n",
    "which is the dispersion relation, meaning that $u(t, x, y) = e^{i(k_x x + k_y y - \\omega t)}$ satisfies the wave equation if and only if $\\omega$, $k_x$ and $k_y$ respect this relation.\n"
   ]
  },
  {
   "cell_type": "markdown",
   "id": "a34185f1",
   "metadata": {},
   "source": [
    "## Exercise 1.2.4\n",
    "\n",
    "We now assume $m_x = m_y$ such that $k_x = k_y = k$. A discrete version of (1) is then given by\n",
    "\n",
    "$$\n",
    "u^n_{i,j} = e^{\\imath (kh(i+j) - \\tilde{\\omega} n\\Delta t)}\n",
    "$$\n",
    "\n",
    "where $\\tilde{\\omega}$ is a numerical dispersion coefficient, i.e the numerical approximation of the exact $\\omega$. We want to insert this equation into the discretized eq\n",
    "\n",
    "$$\n",
    "\\frac{u^{n+1}_{i,j} - 2u^n_{i,j} + u^{n-1}_{i, j}}{\\Delta t^2} =\n",
    " c^2 \\left(\\frac{u^n_{i+1,j} - 2u^n_{i,j} + u^n_{i-1, j}}{h^2} + \\frac{u^n_{i,j+1} - 2u^n_{i,j} + u^n_{i, j-1}}{h^2}\\right)\n",
    "$$\n",
    "\n",
    "and show that for CFL number $C = \\frac{1}{\\sqrt{2}}$, we get $\\tilde{\\omega} = \\omega$\n",
    "\n"
   ]
  },
  {
   "cell_type": "markdown",
   "id": "d4bea836",
   "metadata": {},
   "source": [
    "By inserting the discrete $u_{i,j}^n$ into the scheme, we get\n",
    "\n",
    "$$\n",
    "u_{i,j}^{n+1} = e^{-\\imath \\tilde{\\omega} \\Delta t} u_{i,j}^n,\n",
    "$$\n",
    "$$\n",
    "u_{i,j}^{n-1} = e^{\\imath \\tilde{\\omega} \\Delta t} u_{i,j}^n,\n",
    "$$\n",
    "$$\n",
    "u_{i+1, j}^n = e^{\\imath kh} u_{i,j}^n,\n",
    "$$\n",
    "$$\n",
    "u_{i-1, j}^n = e^{-\\imath kh} u_{i,j}^n,\n",
    "$$\n",
    "$$\n",
    "u_{i, j+1}^n = e^{\\imath kh} u_{i,j}^n,\n",
    "$$\n",
    "$$\n",
    "u_{i, j-1}^n = e^{-\\imath kh} u_{i,j}^n.\n",
    "$$\n",
    "\n",
    "We will then use the identity $e^{\\imath \\theta} + e^{-\\imath \\theta} = 2\\cos(\\theta)$ to write the difference:\n",
    "\n",
    "$$\n",
    "\\frac{e^{-\\imath \\tilde{\\omega} \\Delta t} u_{i,j}^n -2u_{i,j}^n + e^{\\imath \\tilde{\\omega} \\Delta t} u_{i,j}^n}{\\Delta t^2} = c^2(\\frac{e^{\\imath kh} u_{i,j}^n -2u_{i,j}^n + e^{-\\imath kh} u_{i,j}^n}{h^2} + \\frac{e^{\\imath kh} u_{i,j}^n - 2u_{i,j}^n + e^{-\\imath kh} u_{i,j}^n}{h^2}).\n",
    "$$\n",
    "\n",
    "which yields\n",
    "\n",
    "$$\n",
    "u_{i,j}^n \\frac{e^{-\\imath \\tilde{\\omega} \\Delta t} + e^{\\imath \\tilde{\\omega} \\Delta t} - 2}{\\Delta t^2} = 2 c^2 u_{i,j}^n(\\frac{e^{\\imath kh} + e^{-\\imath kh} - 2}{h^2}).\n",
    "$$\n",
    "\n",
    "We then apply the identity. Since $u_{i,j}^n$ never is 0, we divide by $u_{i, j}^n$ on both sides, which yields:\n",
    "\n",
    "$$\n",
    "\\frac{2(\\cos(\\tilde{\\omega} \\Delta t) - 1)}{\\Delta t^2} = 2c^2 \\frac{(2\\cos(kh)-2)}{h^2}.\n",
    "$$\n",
    "\n",
    "We now divide by a factor of 2 and multiply by a factor of $\\Delta t^2$\n",
    "\n",
    "$$\n",
    "\\cos(\\tilde{\\omega} \\Delta t) - 1 = (\\frac{c \\Delta t}{h})^2 (2\\cos(kh)-2),\n",
    "$$\n",
    "\n",
    "and we let $C = \\frac{c \\Delta t}{h}$ and factor out 2 in the RHS, which yields:\n",
    "\n",
    "$$\n",
    "\\cos(\\tilde{\\omega} \\Delta t) - 1 = 2C^2 (\\cos(kh)-1).\n",
    "$$\n",
    "\n",
    "We can now choose $C = \\frac{1}{\\sqrt{2}} \\Rightarrow C^2=\\frac12$, which gives us:\n",
    "\n",
    "$$\n",
    "\\cos(\\tilde{\\omega} \\Delta t) - 1 = \\cos(kh)-1,\n",
    "$$\n",
    "\n",
    "which simplifies to\n",
    "\n",
    "$$\n",
    "\\cos(\\tilde{\\omega} \\Delta t) = \\cos(kh) \\Rightarrow \\tilde{\\omega} \\Delta t = kh\n",
    "$$\n",
    "\n",
    "We know from the continuous case that\n",
    "\n",
    "$$\n",
    "\\omega = c\\sqrt{k_x^2 + k_y^2}\n",
    "$$\n",
    "\n",
    "and we know by assumption that $k_x=k_y=k$, which gives\n",
    "\n",
    "$$\n",
    "\\omega = c\\sqrt{2k^2} = c\\sqrt{2}k.\n",
    "$$\n",
    "\n",
    "so we have\n",
    "\n",
    "$$\n",
    "\\omega \\Delta t = c\\sqrt{2}k \\Delta t = \\sqrt{2}(c \\Delta t)k = \\sqrt{2}C (kh),\n",
    "$$\n",
    "\n",
    "and given that C = $\\frac{1}{\\sqrt{2}}$, we get\n",
    "\n",
    "$$\n",
    "\\omega \\Delta t = kh.\n",
    "$$\n",
    "\n",
    "Hence $\\tilde{\\omega} = \\omega$"
   ]
  }
 ],
 "metadata": {
  "kernelspec": {
   "display_name": "mat-mek4270",
   "language": "python",
   "name": "python3"
  },
  "language_info": {
   "codemirror_mode": {
    "name": "ipython",
    "version": 3
   },
   "file_extension": ".py",
   "mimetype": "text/x-python",
   "name": "python",
   "nbconvert_exporter": "python",
   "pygments_lexer": "ipython3",
   "version": "3.13.7"
  }
 },
 "nbformat": 4,
 "nbformat_minor": 5
}
